Deduction thm with AnyReasoning

matching-logic/src/ProofMode.v
@@ -14,3 +14,172 @@ From MatchingLogic Require Export
 Open Scope ml_scope.
 Open Scope string_scope.
 Open Scope list_scope.
+
+From Coq Require Import String.
+
+Import
+  MatchingLogic.Logic.Notations
+  MatchingLogic.DerivedOperators_Syntax.Notations
+.
+
+Fixpoint proof_size {Σ : Signature} {φ : Pattern} {Γ}
+   (pf : ML_proof_system Γ φ) : nat :=
+match pf with
+ | Modus_ponens _ phi1 phi2 x x0 => 1 + proof_size x + proof_size x0
+ | ProofSystem.Ex_gen _ phi1 phi2 x x0 x1 x2 x3 => 1 + proof_size x2
+ | ProofSystem.Framing_left _ phi1 phi2 psi x x0 => 1 + proof_size x0
+ | ProofSystem.Framing_right _ phi1 phi2 psi x x0 => 1 + proof_size x0
+ | ProofSystem.Svar_subst _ phi psi X x x0 x1 => 1 + proof_size x1
+ | ProofSystem.Knaster_tarski _ phi psi x x0 => 1 + proof_size x0
+ | ProofSystem.Existence _ => 1
+ | _ => 1
+end.
+
+Definition proof_size_info {Σ : Signature} {φ Γ i} (pf : derives_using Γ φ i) : nat :=
+match pf with
+ | exist _ x x0 => proof_size x
+end.
+
+Lemma ex1_coq :
+  forall (A B : Prop), A -> B -> A /\ B.
+Proof.
+  intros. split. assumption. assumption.
+Qed.
+
+(** Low-level proof, using only the proof system *)
+Lemma ex1_low : forall {Σ : Signature} (Γ : Theory) (A B : Pattern),
+  well_formed A = true ->
+  well_formed B = true ->
+  Γ ⊢i (A ---> B ---> (A and B))
+  using BasicReasoning.
+Proof.
+  intros Σ Γ A B WFA WFB.
+  epose proof (tB := (A_impl_A Γ B _)).
+  epose proof (t1 := MP (P2 Γ (!(!A) ---> !B) A Bot _ _ _) (P1 _ _ B _ _)).
+  epose proof (t2 := MP (reorder_meta _ _ _ (P4 Γ (!A) B _ _)) (P1 _ _ B _ _)).
+  epose proof (t3'' := MP (P1 Γ A (!(!A) ---> !B) _ _) (P1 _ _ B _ _)).
+  epose proof (t4 := MP tB (MP t2 (P2 Γ B B _ _ _ _))).
+  epose proof (t5'' := 
+          MP t4
+                       (MP t1
+                                     (P2 Γ B ((!(!A) ---> !B) ---> !A)
+                                         (((!(!A) ---> !B) ---> A) ---> !(!(!A) ---> !B)) _ _ _))).
+  epose proof (tA := (P1 Γ A B) _ _).
+  epose proof (tB' := MP tB (P1 _ (B ---> B) A _ _)).
+  epose proof (t3' := MP t3'' (P2 _ B A ((!(!A) ---> !B) ---> A) _ _ _)).
+  epose proof (t3 := MP t3' (P1 _ ((B ---> A) ---> B ---> (! (! A) ---> ! B) ---> A) A _ _)).
+  epose proof (t5' := MP t5''
+                            (P2 _ B ((!(!A) ---> !B) ---> A) (!(!(!A) ---> !B)) _ _ _)).
+  epose proof (t5 := MP t5' 
+                           (P1 _ ((B ---> (! (! A) ---> ! B) ---> A) ---> B ---> ! (! (! A) ---> ! B))
+                               A _ _)).
+  epose proof (t6 := MP tA
+                           (MP t3
+                                         (P2 _ A (B ---> A) (B ---> (!(!A) ---> !B) ---> A) _ _ _))).
+  epose proof (t7 := MP t6 
+                           (MP t5 
+                                         (P2 _ A (B ---> (!(!A) ---> !B) ---> A) (B ---> !(!(!A) ---> !B)) _ _ _))).
+  apply t7.
+  Unshelve.
+    (* 43 well-formedness goals *)
+    all: wf_auto2.
+Defined.
+
+From Coq Require Import ssreflect ssrfun ssrbool.
+
+Open Scope string_scope.
+Open Scope list_scope.
+Open Scope ml_scope.
+
+Lemma ex1_pm2 : forall {Σ : Signature} (Γ : Theory) (A B : Pattern),
+  well_formed A = true ->
+  well_formed B = true ->
+  Γ ⊢i (A ---> B ---> (A and B))
+  using BasicReasoning.
+Proof.
+  intros Σ Γ A B WFA WFB.
+  do 2 mlIntro; mlSplitAnd; mlAssumption.
+Defined.
+
+(** Proof using proof mode *)
+Lemma ex1_pm : forall {Σ : Signature} (Γ : Theory) (A B : Pattern),
+  well_formed A = true ->
+  well_formed B = true ->
+  Γ ⊢i (A ---> B ---> (A and B))
+  using BasicReasoning.
+Proof.
+  intros Σ Γ A B WFA WFB.
+  unfold patt_and, patt_or, patt_not.
+  mlIntro "Ha". mlIntro "Hb". mlIntro "H".
+  mlAssert ("H0" : B). { wf_auto2. } { mlAssumption. }
+  mlRevertLast.
+  mlApply "H".
+  mlIntro "H0". mlApply "H0". mlAssumption.
+Defined.
+
+Section compute.
+  From MatchingLogic.Theories Require Import Definedness_Syntax
+                                             Definedness_Semantics
+                                             Sorts_Syntax
+                                             Sorts_Semantics
+                                             Definedness_ProofSystem.
+  From stdpp Require Import base fin_sets sets propset finite.
+
+  Inductive Symbols :=
+    | sym_import_definedness (d : Definedness_Syntax.Symbols)
+    | Zero | Succ (* constructors for Nats *)
+    | TT | FF
+    | even
+  .
+
+  Instance Symbols_eqdec : EqDecision Symbols.
+  Proof. solve_decision. Defined.
+
+  #[local]
+  Program Instance Symbols_fin : Finite Symbols :=
+  {|
+    enum := [Zero; Succ; TT ; FF; even;
+      sym_import_definedness Definedness_Syntax.definedness] ;
+  |}.
+  Next Obligation.
+    repeat constructor; set_solver.
+  Qed.
+  Next Obligation.
+    destruct x; try set_solver.
+    destruct d; set_solver.
+  Qed.
+
+  Instance signature : Signature :=
+    {| variables := StringMLVariables ;
+       symbols := Symbols ;
+    |}.
+
+  Instance definedness_syntax : Definedness_Syntax.Syntax :=
+    {|
+       Definedness_Syntax.inj := sym_import_definedness;
+    |}.
+
+  Open Scope string_scope.
+  Let X0 := patt_free_evar "X0".
+  Let X := patt_free_evar "X".
+  Let sym_even := patt_sym even.
+  Let sym_succ := patt_sym Succ.
+  Let sym_zero := patt_sym Zero.
+  Let sym_tt := patt_sym TT.
+  Let sym_ff := patt_sym FF.
+  (* axioms *)
+  Definition defined : Pattern := Definedness_Syntax.axiom AxDefinedness.
+
+  Definition A : Pattern :=
+    sym_zero.
+  Definition B : Pattern :=
+    patt_app sym_succ sym_zero.
+
+  Definition proof1_low : nat := proof_size_info (ex1_low ∅ A B ltac:(wf_auto2) ltac:(wf_auto2)).
+  Definition proof1_pm : nat := proof_size_info (ex1_pm ∅ A B ltac:(wf_auto2) ltac:(wf_auto2)).
+  Definition proof1_pm2 : nat := proof_size_info (ex1_pm2 ∅ A B ltac:(wf_auto2) ltac:(wf_auto2)).
+(*
+  Compute proof_size_info (ex1_low ∅ A B ltac:(wf_auto2) ltac:(wf_auto2)).
+  Compute proof_size_info (ex1_pm ∅ A B ltac:(wf_auto2) ltac:(wf_auto2)). *)
+
+End compute.
